backend/Allocproof.v
@@ -2444,7 +2444,7 @@ Proof.
 (* internal function *)
 - monadInv FUN. simpl in *.
   destruct (transf_function_inv _ _ EQ).
-  exploit Mem.alloc_extends; eauto. apply Zle_refl. rewrite H8; apply Zle_refl.
+  exploit Mem.alloc_extends; eauto. apply Z.le_refl. rewrite H8; apply Z.le_refl.
   intros [m'' [U V]].
   assert (WTRS: wt_regset env (init_regs args (fn_params f))).
   { apply wt_init_regs. inv H0. rewrite wt_params. rewrite H9. auto. }
